added counting code

paper-code/SchulzeSynthesis.v
@@ -644,3 +644,139 @@ Section Evote.
   
 End Evote.
 
+(* Start of ballot counting code *)
+Section Count.
+
+  
+  Hypothesis cand_fin : forall c: cand, In c cand_all.
+  Hypothesis dec_cand : forall n m : cand, {n = m} + {n <> m}.
+  Hypothesis cand_not_nil : cand_all <> nil.
+
+  Definition ballot := cand -> nat.
+
+  (* ballot is valid if foreach candidate there is number greater than zero *)
+  Definition ballot_valid (p : ballot) : Prop :=
+    forall c : cand, (p c > 0)%nat.
+
+  Inductive Node : Type :=
+  | state : (list ballot * list ballot)  -> (cand -> cand -> Z) -> Node
+  | winners : (cand -> bool) ->  Node.
+  
+  (* earlier c d p means that c occurs earlier in the ballot p *)
+  Definition earlier (c d : cand) (p : ballot) : Prop :=
+    (p c > 0)%nat /\ (p d > 0)%nat /\ (p c < p d)%nat.
+
+  (* equal c d p means that both c and d have same rank/preference in ballot p *)
+  Definition equal (c d : cand) (p : ballot) : Prop :=
+    (p c > 0)%nat /\ (p d > 0)%nat /\ (p c = p d)%nat.
+
+  Theorem in_decidable :
+    forall (b : ballot) (l : list cand),
+      {forall c : cand, In c l -> (b c > 0)%nat} + {~(forall c : cand, In c l -> (b c > 0)%nat)}.
+  Proof.
+    intros b. induction l.
+    left. intros. inversion H. 
+    destruct IHl. destruct (le_gt_dec (b a) 0) as [H1 | H2].
+    right. intro. pose proof (H a (or_introl eq_refl)). omega.
+    left. firstorder. subst. assumption.
+    right. firstorder.
+  Qed.
+
+  (* each ballot is either valid or invalid *)
+  Lemma valid_or_invalid_ballot : forall b : ballot, {ballot_valid b} + {~ballot_valid b}.
+  Proof.
+    intros b. pose proof in_decidable b cand_all.
+    destruct H; [left | right]; firstorder. 
+  Qed.
+
+  (* null tally *)
+  Definition nty (c d : cand) := 0%Z.
+
+  Definition incdec (c d : cand) (t: cand -> cand -> Z)
+             (nt : cand -> cand -> Z) : Prop :=
+    (nt c d = t c d + 1)%Z /\
+    (nt d c = t d c - 1)%Z.
+
+  Definition nochange (c d : cand) (t : cand -> cand -> Z)
+             (nt : cand -> cand -> Z) : Prop :=
+    nt c d = t c d.
+  
+  Inductive Count (bs : list ballot) : Node -> Type :=
+  | ax us t : us = bs -> t = nty -> Count bs (state (us, []) t)
+  | cvalid u us m nm inbs :
+      Count bs (state (u :: us, inbs) m) -> ballot_valid u -> 
+      (forall c d : cand, (earlier c d u -> incdec c d m nm) /\
+                     (equal c d u -> nochange c d m nm)) ->
+      Count bs (state (us, inbs) nm)
+  | cinvalid u us m inbs :
+      Count bs (state (u :: us, inbs) m) -> ~(ballot_valid u) ->
+      Count bs (state (us, u :: inbs) m)
+  | fin m inbs w (d : (forall c, (wins_type m c) + (loses_type m c))):
+      Count bs (state ([], inbs) m) ->
+      (forall c, w c = true <-> (exists x, d c = inl x)) ->
+      (forall c, w c = false <-> (exists x, d c = inr x)) ->
+      Count bs (winners w).
+
+  Definition incdect (p : ballot) (m : cand -> cand -> Z) :
+    cand -> cand -> Z :=
+    fun c d =>
+      match nat_compare_alt (p c) (p d) with
+      | Lt => (m c d + 1)%Z
+      | Eq => m c d
+      | Gt => (m c d - 1)%Z
+      end.
+  
+  
+  Lemma incdec_proof : forall m (p : ballot) (c d : cand),
+      (earlier c d p -> incdec c d m (incdect p m)) /\
+      (equal c d p -> nochange c d m (incdect p m)).
+  Proof.
+    intros m p c d. split; intros.
+    unfold earlier in H. unfold incdec. unfold incdect.
+    destruct H as [H1 [H2 H3]]. split.
+    unfold nat_compare_alt. destruct (lt_eq_lt_dec (p c) (p d)) eqn:H.
+    destruct s. auto. omega. omega.
+    unfold nat_compare_alt. destruct (lt_eq_lt_dec (p d) (p c)) eqn:H.
+    destruct s. omega. omega. auto.
+    unfold equal in H. destruct H as [H1 [H2 H3]].
+    unfold nochange, incdect, nat_compare_alt.
+    rewrite H3. destruct (lt_eq_lt_dec (p d) (p d)) eqn:H.
+    destruct s; omega. omega.
+  Qed.
+  
+  Lemma extract_prog_gen : forall bs u inbs m,
+      Count bs (state (u, inbs) m) -> existsT i m, (Count bs (state ([], i) m)).
+  Proof.
+    intros bs. induction u.
+    intros. exists inbs, m. auto.
+    pose proof valid_or_invalid_ballot a.
+    destruct H; swap 1 2. intros.
+    pose proof (cinvalid bs a u m inbs X n).
+    specialize (IHu (a :: inbs) m X0).
+    destruct IHu as [Hinv [Hmar H3]].
+    exists Hinv, Hmar. assumption.
+    intros. pose proof (cvalid bs a u m (incdect a m) inbs X b (incdec_proof m a)).
+    specialize (IHu inbs (incdect a m) X0). destruct IHu as [Hinv [Hm H]].
+    exists Hinv, Hm. assumption.
+  Defined.
+
+  Lemma extract_prog :
+    forall (bs : list ballot), existsT i m, (Count bs (state ([], i) m)). 
+  Proof.
+    intros bs.
+    pose proof (extract_prog_gen bs bs [] nty (ax bs bs nty eq_refl eq_refl)).
+    destruct X as [i [m Hc]].
+    exists i, m. assumption.
+  Defined.
+
+  Lemma final_count : forall (bs : list ballot), existsT (f : cand -> bool) (p : Count bs (winners f)), True.
+  Proof.
+    intros. pose proof (extract_prog bs). destruct X as [bs' [m X]].
+    pose proof (fin bs _ bs' (c_wins m) (wins_loses_M cand_fin dec_cand cand_not_nil m) X).
+    pose proof (X0 (winner_one cand_fin dec_cand cand_not_nil m)
+                   (loser_one cand_fin dec_cand cand_not_nil m)).
+    exists (c_wins m). exists X1. apply I.
+  Defined.
+
+End Count.
+
